specs/L1AssetRouter/L1AssetRouter/Common/if_6182723117196027006_user.lean
@@ -12,12 +12,14 @@ section
 
 open Clear EVMState Ast Expr Stmt FunctionDefinition State Interpreter ExecLemmas OutOfFuelLemmas Abstraction YulNotation PrimOps ReasoningPrinciple Utilities generated.L1AssetRouter L1AssetRouter
 
-def A_if_6182723117196027006 (s₀ s₉ : State) : Prop := sorry
+def A_if_6182723117196027006 (s₀ s₉ : State) : Prop :=
+  if_6182723117196027006_concrete_of_code.1 s₀ s₉
 
 lemma if_6182723117196027006_abs_of_concrete {s₀ s₉ : State} :
   Spec if_6182723117196027006_concrete_of_code s₀ s₉ →
   Spec A_if_6182723117196027006 s₀ s₉ := by
-  sorry
+  intro h
+  simpa [A_if_6182723117196027006] using h
 
 end
 
